split stdlib Program into Init and deprecated

theories/Program/Basics.v
@@ -8,53 +8,17 @@
 (*         *     GNU Lesser General Public License Version 2.1          *)
 (*         *     (see LICENSE file for the text of the license)         *)
 (************************************************************************)
-(** Standard functions and combinators.
-
-   Proofs about them require functional extensionality and can be found
-   in [Combinators].
-
-   Author: Matthieu Sozeau
-   Institution: LRI, CNRS UMR 8623 - University Paris Sud
-*)
-
-(** The polymorphic identity function is defined in [Datatypes]. *)
-
-Arguments id {A} x.
-
-(** Function composition. *)
-
-Definition compose {A B C} (g : B -> C) (f : A -> B) :=
-  fun x : A => g (f x).
-
-#[global]
-Hint Unfold compose : core.
-
-Declare Scope program_scope.
-
-Notation " g ∘ f " := (compose g f)
-  (at level 40, left associativity) : program_scope.
-
-Local Open Scope program_scope.
-
-(** The non-dependent function space between [A] and [B]. *)
-
-Definition arrow (A B : Type) := A -> B.
-Register arrow as core.arrow.
-
-(** Logical implication. *)
-
-Definition impl (A B : Prop) : Prop := A -> B.
-Register impl as core.impl.
-
-(** The constant function [const a] always returns [a]. *)
-
-Definition const {A B} (a : A) := fun _ : B => a.
-
-(** The [flip] combinator reverses the first two arguments of a function. *)
-
-Definition flip {A B C} (f : A -> B -> C) x y := f y x.
-Register flip as core.flip.
-
-(** Application as a combinator. *)
-
-Definition apply {A B} (f : A -> B) (x : A) := f x.
+Attributes deprecated(since="9.0", note="use Init.Basics").
+Require Export Init.Basics.
+#[deprecated(use=compose, since="9.0")]
+Notation compose := compose (only parsing).
+#[deprecated(use=arrow, since="9.0")]
+Notation arrow := arrow (only parsing).
+#[deprecated(use=impl, since="9.0")]
+Notation impl := impl (only parsing).
+#[deprecated(use=const, since="9.0")]
+Notation const := const (only parsing).
+#[deprecated(use=flip, since="9.0")]
+Notation flip := flip (only parsing).
+#[deprecated(use=apply, since="9.0")]
+Notation apply := apply (only parsing).
