theories/Program/Wf.v
@@ -1,258 +1,49 @@
-(************************************************************************)
-(*         *      The Rocq Prover / The Rocq Development Team           *)
-(*  v      *         Copyright INRIA, CNRS and contributors             *)
-(* <O___,, * (see version control and CREDITS file for authors & dates) *)
-(*   \VV/  **************************************************************)
-(*    //   *    This file is distributed under the terms of the         *)
-(*         *     GNU Lesser General Public License Version 2.1          *)
-(*         *     (see LICENSE file for the text of the license)         *)
-(************************************************************************)
-(** Reformulation of the Wf module using subsets where possible, providing
-   the support for [Program]'s treatment of well-founded definitions. *)
+Attributes deprecated(since="9.0", note="use Init.Wf").
 
-Require Import Stdlib.Init.Wf.
-Require Import Stdlib.Program.Utils.
+Require Export Stdlib.Init.Wf.
 
-Local Open Scope program_scope.
+#[deprecated(use=Fix_F_sub, since="9.0")]
+Notation Fix_F_sub := Fix_F_sub (only parsing).
 
-Section Well_founded.
-  Variable A : Type.
-  Variable R : A -> A -> Prop.
-  Hypothesis Rwf : well_founded R.
+#[deprecated(use=Fix_sub, since="9.0")]
+Notation Fix_sub := Fix_sub (only parsing).
 
-  Variable P : A -> Type.
+#[deprecated(use=Fix_F_eq, since="9.0")]
+Notation Fix_F_eq := Fix_F_sub_eq (only parsing).
 
-  Variable F_sub : forall x:A, (forall y: { y : A | R y x }, P (proj1_sig y)) -> P x.
+#[deprecated(use=Fix_F_inv, since="9.0")]
+Notation Fix_F_inv := Fix_F_sub_inv (only parsing).
 
-  Fixpoint Fix_F_sub (x : A) (r : Acc R x) : P x :=
-    F_sub x (fun y: { y : A | R y x}  => Fix_F_sub (proj1_sig y)
-      (Acc_inv r (proj2_sig y))).
+#[deprecated(use=Fix_eq, since="9.0")]
+Notation Fix_eq := Fix_sub_eq (only parsing).
 
-  Definition Fix_sub (x : A) := Fix_F_sub x (Rwf x).
+#[deprecated(use=MR, since="9.0")]
+Notation MR := MR (only parsing).
 
-  Register Fix_sub as program.wf.fix_sub.
+#[deprecated(use=measure_wf, since="9.0")]
+Notation measure_wf := measure_wf (only parsing).
 
-  (* Notation Fix_F := (Fix_F_sub P F_sub) (only parsing). (* alias *) *)
-  (* Definition Fix (x:A) := Fix_F_sub P F_sub x (Rwf x). *)
+#[deprecated(use=F_unfold, since="9.0")]
+Notation F_unfold := F_unfold (only parsing).
 
-  Hypothesis F_ext :
-    forall (x:A) (f g:forall y:{y:A | R y x}, P (`y)),
-      (forall y:{y : A | R y x}, f y = g y) -> F_sub x f = F_sub x g.
+#[deprecated(use=Fix_F_sub_rect, since="9.0")]
+Notation Fix_F_sub_rect:= Fix_F_sub_rect(only parsing).
 
-  Lemma Fix_F_eq :
-    forall (x:A) (r:Acc R x),
-      F_sub x (fun y:{y:A | R y x} => Fix_F_sub (`y) (Acc_inv r (proj2_sig y))) = Fix_F_sub x r.
-  Proof.
-    intros x r; destruct r using Acc_inv_dep; auto.
-  Qed.
+#[deprecated(use=eq_Fix_F_sub, since="9.0")]
+Notation eq_Fix_F_sub := eq_Fix_F_sub (only parsing).
 
-  Lemma Fix_F_inv : forall (x:A) (r s:Acc R x), Fix_F_sub x r = Fix_F_sub x s.
-  Proof.
-    intro x; induction (Rwf x); intros.
-    rewrite <- 2 Fix_F_eq; intros. apply F_ext; intros []; auto.
-  Qed.
+#[deprecated(use=Fix_sub_rect, since="9.0")]
+Notation Fix_sub_rect:= Fix_sub_rect(only parsing).
 
-  Lemma Fix_eq : forall x:A, Fix_sub x = F_sub x (fun y:{ y:A | R y x} => Fix_sub (proj1_sig y)).
-  Proof.
-    intro x; unfold Fix_sub.
-    rewrite <- (Fix_F_eq ).
-    apply F_ext; intros.
-    apply Fix_F_inv.
-  Qed.
+#[deprecated(Note="Use Init.Wf.fold_sub", since="9.0")]
+Ltac fold_sub := fold_sub.
 
-  Lemma fix_sub_eq :
-    forall x : A,
-      Fix_sub x =
-      let f_sub := F_sub in
-        f_sub x (fun y: {y : A | R y x} => Fix_sub (`y)).
-  Proof.
-    exact Fix_eq.
-  Qed.
-
-End Well_founded.
-
-Require Stdlib.extraction.Extraction.
-Extraction Inline Fix_F_sub Fix_sub.
-
-Set Implicit Arguments.
-
-(** Reasoning about well-founded fixpoints on measures. *)
-
-Section Measure_well_founded.
-
-  (* Measure relations are well-founded if the underlying relation is well-founded. *)
-
-  Variables T M: Type.
-  Variable R: M -> M -> Prop.
-  Hypothesis wf: well_founded R.
-  Variable m: T -> M.
-
-  Definition MR (x y: T): Prop := R (m x) (m y).
-
-  Register MR as program.wf.mr.
-
-  Lemma measure_wf: well_founded MR.
-  Proof with auto.
-    unfold well_founded.
-    cut (forall (a: M) (a0: T), m a0 = a -> Acc MR a0).
-    + intros H a.
-      apply (H (m a))...
-    + apply (@well_founded_ind M R wf (fun mm => forall a, m a = mm -> Acc MR a)).
-      intros ? H ? H0.
-      apply Acc_intro.
-      intros y H1.
-      unfold MR in H1.
-      rewrite H0 in H1.
-      apply (H (m y))...
-  Defined.
-
-End Measure_well_founded.
-
-#[global]
-Hint Resolve measure_wf : core.
-
-Section Fix_rects.
-
-  Variable A: Type.
-  Variable P: A -> Type.
-  Variable R : A -> A -> Prop.
-  Variable Rwf : well_founded R.
-  Variable f: forall (x : A), (forall y: { y: A | R y x }, P (proj1_sig y)) -> P x.
-
-  Lemma F_unfold x r:
-    Fix_F_sub A R P f x r =
-    f (fun y => Fix_F_sub A R P f (proj1_sig y) (Acc_inv r (proj2_sig y))).
-  Proof. intros. case r; auto. Qed.
-
-  (* Fix_F_sub_rect lets one prove a property of
-  functions defined using Fix_F_sub by showing
-  that property to be invariant over single application of the
-  function body (f in our case). *)
-
-  Lemma Fix_F_sub_rect
-    (Q: forall x, P x -> Type)
-    (inv: forall x: A,
-     (forall (y: A) (H: R y x) (a: Acc R y),
-        Q y (Fix_F_sub A R P f y a)) ->
-        forall (a: Acc R x),
-          Q x (f (fun y: {y: A | R y x} =>
-            Fix_F_sub A R P f (proj1_sig y) (Acc_inv a (proj2_sig y)))))
-    : forall x a, Q _ (Fix_F_sub A R P f x a).
-  Proof with auto.
-    set (R' := fun (x: A) => forall a, Q _ (Fix_F_sub A R P f x a)).
-    cut (forall x, R' x)...
-    apply (well_founded_induction_type Rwf).
-    subst R'.
-    simpl.
-    intros.
-    rewrite F_unfold...
-  Qed.
-
-  (* Let's call f's second parameter its "lowers" function, since it
-  provides it access to results for inputs with a lower measure.
-
-  In preparation of lemma similar to Fix_F_sub_rect, but
-  for Fix_sub, we first
-  need an extra hypothesis stating that the function body has the
-  same result for different "lowers" functions (g and h below) as long
-  as those produce the same results for lower inputs, regardless
-  of the lt proofs. *)
-
-  Hypothesis equiv_lowers:
-    forall x0 (g h: forall x: {y: A | R y x0}, P (proj1_sig x)),
-    (forall x p p', g (exist (fun y: A => R y x0) x p) = h (exist (*FIXME shouldn't be needed *) (fun y => R y x0) x p')) ->
-      f g = f h.
-
-  (* From equiv_lowers, it follows that
-   [Fix_F_sub A R P f x] applications do not not
-  depend on the Acc proofs. *)
-
-  Lemma eq_Fix_F_sub x (a a': Acc R x):
-    Fix_F_sub A R P f x a =
-    Fix_F_sub A R P f x a'.
-  Proof.
-    revert a'.
-    pattern x, (Fix_F_sub A R P f x a).
-    apply Fix_F_sub_rect.
-    intros ? H **.
-    rewrite F_unfold.
-    apply equiv_lowers.
-    intros.
-    apply H.
-    assumption.
-  Qed.
-
-  (* Finally, Fix_F_rect lets one prove a property of
-  functions defined using Fix_F_sub by showing that
-  property to be invariant over single application of the function
-  body (f). *)
-
-  Lemma Fix_sub_rect
-    (Q: forall x, P x -> Type)
-    (inv: forall
-      (x: A)
-      (H: forall (y: A), R y x -> Q y (Fix_sub A R Rwf P f y))
-      (a: Acc R x),
-        Q x (f (fun y: {y: A | R y x} => Fix_sub A R Rwf P f (proj1_sig y))))
-    : forall x, Q _ (Fix_sub A R Rwf P f x).
-  Proof with auto.
-    unfold Fix_sub.
-    intros x.
-    apply Fix_F_sub_rect.
-    intros x0 H a.
-    assert (forall y: A, R y x0 -> Q y (Fix_F_sub A R P f y (Rwf y))) as X0...
-    set (q := inv x0 X0 a). clearbody q.
-    rewrite <- (equiv_lowers (fun y: {y: A | R y x0} =>
-      Fix_F_sub A R P f (proj1_sig y) (Rwf (proj1_sig y)))
-    (fun y: {y: A | R y x0} => Fix_F_sub A R P f (proj1_sig y) (Acc_inv a (proj2_sig y))))...
-    intros.
-    apply eq_Fix_F_sub.
-  Qed.
-
-End Fix_rects.
-
-(** Tactic to fold a definition based on [Fix_measure_sub]. *)
-
-Ltac fold_sub f :=
-  match goal with
-    | [ |- ?T ] =>
-      match T with
-        context C [ @Fix_sub _ _ _ _ _ ?arg ] =>
-        let app := context C [ f arg ] in
-          change app
-      end
-  end.
-
-(** This module provides the fixpoint equation provided one assumes
-   functional extensionality. *)
-Require Import FunctionalExtensionality.
+Require Import FunctionalExtensionalityWf.
 
 Module WfExtensionality.
-
-  (** The two following lemmas allow to unfold a well-founded fixpoint definition without
-     restriction using the functional extensionality axiom. *)
-
-  (** For a function defined with Program using a well-founded order. *)
-
-  Lemma fix_sub_eq_ext :
-    forall (A : Type) (R : A -> A -> Prop) (Rwf : well_founded R)
-      (P : A -> Type)
-      (F_sub : forall x : A, (forall y:{y : A | R y x}, P (` y)) -> P x),
-      forall x : A,
-        Fix_sub A R Rwf P F_sub x =
-          F_sub x (fun y:{y : A | R y x} => Fix_sub A R Rwf P F_sub (` y)).
-  Proof.
-    intros A R Rwf P F_sub x; apply Fix_eq ; auto.
-    intros ? f g H.
-    assert(f = g) as H0.
-    - extensionality y ; apply H.
-    - rewrite H0 ; auto.
-  Qed.
-
-  (** Tactic to unfold once a definition based on [Fix_sub]. *)
-
-  Ltac unfold_sub f fargs :=
-    set (call:=fargs) ; unfold f in call ; unfold call ; clear call ;
-      rewrite fix_sub_eq_ext ; repeat fold_sub f ; simpl proj1_sig.
-
+  #[deprecated(use=fix_sub_eq_ext, since="9.0")]
+  Notation fix_sub_eq_ext := fix_sub_eq_ext (only parsing).
+  
+  #[deprecated(Note="Use Init.Wf.fold_sub", since="9.0")]
+  Ltac unfold_sub := FunctionalExtensionalityWf.unfold_sub.
 End WfExtensionality.
