theories/Logic/FunctionalExtensionalityWf.v
@@ -1,0 +1,21 @@
+Require Import FunctionalExtensionality.
+Require Import Init.Wf.
+
+Lemma fix_sub_eq_ext :
+  forall (A : Type) (R : A -> A -> Prop) (Rwf : well_founded R)
+    (P : A -> Type)
+    (F_sub : forall x : A, (forall y:{y : A | R y x}, P (proj1_sig y)) -> P x),
+    forall x : A,
+      Fix_sub A R Rwf P F_sub x =
+        F_sub x (fun y:{y : A | R y x} => Fix_sub A R Rwf P F_sub (proj1_sig y)).
+Proof.
+  intros A R Rwf P F_sub x; apply Fix_sub_eq ; auto.
+  intros ? f g H.
+  assert(f = g) as H0.
+  - extensionality y ; apply H.
+  - rewrite H0 ; auto.
+Qed.
+
+Ltac unfold_sub f fargs :=
+  set (call:=fargs) ; unfold f in call ; unfold call ; clear call ;
+    rewrite fix_sub_eq_ext ; repeat fold_sub f ; simpl proj1_sig.
