theories/Program/Tactics.v
@@ -7,6 +7,7 @@
 (*         *     GNU Lesser General Public License Version 2.1          *)
 (*         *     (see LICENSE file for the text of the license)         *)
 (************************************************************************)
+Attributes deprecated(since="9.0").
 
 (** This module implements various tactics used to simplify the goals produced by Program,
    which are also generally useful. *)
